src/protocol/DNS.Protocol.Parser.EverParseAdapter.fst
@@ -18,6 +18,8 @@ let generated_dns_two_label_question_validator_linked : bool = true
 
 let generated_dns_uncompressed_question_validator_linked : bool = true
 
+let generated_dns_uncompressed_question_answer_packet_validator_linked : bool = true
+
 let generated_dns_header_validator = DNSProtocol.validate__dns_header
 
 let generated_dns_root_question_validator =
@@ -31,3 +33,6 @@ let generated_dns_two_label_question_validator first_label_length second_label_l
 
 let generated_dns_uncompressed_question_validator qname_length =
   DNSProtocol.validate__dns_uncompressed_question qname_length
+
+let generated_dns_uncompressed_question_answer_packet_validator qname_length rr_name_length rdata_length =
+  DNSProtocol.validate__dns_uncompressed_question_answer_packet qname_length rr_name_length rdata_length
